src/main/isabelle/Tactics.thy
@@ -41,6 +41,70 @@ lemma wp2_sample:
   shows "qrhl A [] [sample x e] B"
   sorry
 
+lemma wp1_qapply:
+  fixes A B Q e
+  defines "A \<equiv> map_expression2 (\<lambda>e\<^sub>1 B. Cla[isometry e\<^sub>1] \<sqinter> (adjoint (e\<^sub>1\<guillemotright>Q) \<cdot> (B \<sqinter> (e\<^sub>1\<guillemotright>Q \<cdot> top)))) (index_expression True e) B"
+  shows "qrhl A [qapply Q e] [] B"
+  sorry
+
+lemma wp2_qapply:
+  fixes A B Q e
+  defines "A \<equiv> map_expression2 (\<lambda>e\<^sub>2 B. Cla[isometry e\<^sub>2] \<sqinter> (adjoint (e\<^sub>2\<guillemotright>Q) \<cdot> (B \<sqinter> (e\<^sub>2\<guillemotright>Q \<cdot> top)))) (index_expression False e) B"
+  shows "qrhl A [] [qapply Q e] B"
+  sorry
+
+lemma wp1_measure:
+  fixes A B x Q e
+  defines "e\<^sub>1 \<equiv> index_expression True e"
+  defines "B' z \<equiv> subst_expression (substitute1 (index_var True x) (const_expression z)) B"
+  defines "\<And>e\<^sub>1 z. ebar e\<^sub>1 z \<equiv> ((mproj e\<^sub>1 z)\<guillemotright>Q) \<cdot> top"
+  defines "A \<equiv> map_expression2' (\<lambda>e\<^sub>1 B'. Cla[mtotal e\<^sub>1] \<sqinter> 
+           (INF z. ((B' z \<sqinter> ebar e\<^sub>1 z) + ortho (ebar e\<^sub>1 z)))) e\<^sub>1 B'"
+  shows "qrhl A [measurement x Q e] [] B"
+  sorry
+
+lemma wp2_measure:
+  fixes A B x Q e
+  defines "e\<^sub>2 \<equiv> index_expression False e"
+  defines "B' z \<equiv> subst_expression (substitute1 (index_var False x) (const_expression z)) B"
+  defines "\<And>e\<^sub>2 z. ebar e\<^sub>2 z \<equiv> ((mproj e\<^sub>2 z)\<guillemotright>Q) \<cdot> top"
+  defines "A \<equiv> map_expression2' (\<lambda>e\<^sub>2 B'. Cla[mtotal e\<^sub>2] \<sqinter> 
+           (INF z. ((B' z \<sqinter> ebar e\<^sub>2 z) + ortho (ebar e\<^sub>2 z)))) e\<^sub>2 B'"
+  shows "qrhl A [measurement x Q e] [] B"
+  sorry
+
+lemma wp1_qinit:
+  fixes B e Q
+  defines "A \<equiv> map_expression2 (\<lambda>e\<^sub>1 B. Cla[norm e\<^sub>1 = 1] \<sqinter> (B \<div> e\<^sub>1 \<guillemotright> Q))
+           (index_expression True e) B"
+  shows "qrhl A [qinit Q e] [] B"
+  sorry
+
+lemma wp2_qinit:
+  fixes B e Q
+  defines "A \<equiv> map_expression2 (\<lambda>e\<^sub>2 B. Cla[norm e\<^sub>2 = 2] \<sqinter> (B \<div> e\<^sub>2 \<guillemotright> Q))
+           (index_expression False e) B"
+  shows "qrhl A [qinit Q e] [] B"
+  sorry
+
+lemma wp1_if:
+  fixes e p1 p2 B
+  assumes "qrhl wp_true p1 [] B"
+  assumes "qrhl wp_false p2 [] B"
+  defines "A \<equiv> map_expression3 (\<lambda>e\<^sub>1 wp_true wp_false. (Cla[e\<^sub>1] + wp_true) \<sqinter> (Cla[\<not>e\<^sub>1] + wp_false))
+           (index_expression True e) wp_true wp_false"
+  shows "qrhl A [ifthenelse e p1 p2] [] B"
+  sorry
+
+lemma wp2_if:
+  fixes e p1 p2 B
+  assumes "qrhl wp_true p1 [] B"
+  assumes "qrhl wp_false p2 [] B"
+  defines "A \<equiv> map_expression3 (\<lambda>e\<^sub>2 wp_true wp_false. (Cla[e\<^sub>2] + wp_true) \<sqinter> (Cla[\<not>e\<^sub>2] + wp_false))
+           (index_expression False e) wp_true wp_false"
+  shows "qrhl A [ifthenelse e p1 p2] [] B"
+  sorry
+
 lemma wp1_block:
   assumes "qrhl A p [] B"
   shows "qrhl A [block p] [] B"
